disk-betree/ImplModelSplit.i.dfy
@@ -25,7 +25,7 @@ module ImplModelSplit {
     var cLeft := Pivots.CutoffForLeft(node.pivotTable, pivot);
     var leftPivots := node.pivotTable[.. cLeft];
     var leftChildren := if node.children.Some? then Some(node.children.value[.. cLeft + 1]) else None;
-    var splitBucket := KMTable.splitLeft(node.buckets[cLeft], pivot);
+    var splitBucket := SplitBucketLeft(node.buckets[cLeft], pivot);
     var leftBuckets := node.buckets[.. cLeft] + [splitBucket];
     Node(leftPivots, leftChildren, leftBuckets)
   }
@@ -42,13 +42,11 @@ module ImplModelSplit {
     var cLeft := Pivots.CutoffForLeft(node.pivotTable, pivot);
     var leftPivots := node.pivotTable[.. cLeft];
     var leftChildren := if node.children.Some? then Some(node.children.value[.. cLeft + 1]) else None;
-    var splitBucket := KMTable.splitLeft(node.buckets[cLeft], pivot);
+    var splitBucket := SplitBucketLeft(node.buckets[cLeft], pivot);
     var leftBuckets := node.buckets[.. cLeft] + [splitBucket];
     Pivots.WFSlice(node.pivotTable, 0, cLeft);
-    KMTable.Islice(node.buckets, 0, cLeft);
-    KMTable.IPopBack(node.buckets[.. cLeft], splitBucket);
-    WFSplitBucketListLeft(KMTable.ISeq(node.buckets), node.pivotTable, cLeft, pivot);
-    WeightSplitBucketListLeft(KMTable.ISeq(node.buckets), node.pivotTable, cLeft, pivot);
+    WFSplitBucketListLeft(node.buckets, node.pivotTable, cLeft, pivot);
+    WeightSplitBucketListLeft(node.buckets, node.pivotTable, cLeft, pivot);
   }
 
   function {:opaque} CutoffNodeAndKeepRight(node: Node, pivot: Key)
@@ -60,7 +58,7 @@ module ImplModelSplit {
     var cRight := Pivots.CutoffForRight(node.pivotTable, pivot);
     var rightPivots := node.pivotTable[cRight ..];
     var rightChildren := if node.children.Some? then Some(node.children.value[cRight ..]) else None;
-    var splitBucket := KMTable.splitRight(node.buckets[cRight], pivot);
+    var splitBucket := SplitBucketRight(node.buckets[cRight], pivot);
     var rightBuckets := [splitBucket] + node.buckets[cRight + 1 ..];
     Node(rightPivots, rightChildren, rightBuckets)
   }
@@ -77,13 +75,11 @@ module ImplModelSplit {
     var cRight := Pivots.CutoffForRight(node.pivotTable, pivot);
     var rightPivots := node.pivotTable[cRight ..];
     var rightChildren := if node.children.Some? then Some(node.children.value[cRight ..]) else None;
-    var splitBucket := KMTable.splitRight(node.buckets[cRight], pivot);
+    var splitBucket := SplitBucketRight(node.buckets[cRight], pivot);
     var rightBuckets := [splitBucket] + node.buckets[cRight + 1 ..];
     Pivots.WFSuffix(node.pivotTable, cRight);
-    KMTable.Isuffix(node.buckets, cRight + 1);
-    KMTable.IPopFront(splitBucket, node.buckets[cRight + 1 ..]);
-    WFSplitBucketListRight(KMTable.ISeq(node.buckets), node.pivotTable, cRight, pivot);
-    WeightSplitBucketListRight(KMTable.ISeq(node.buckets), node.pivotTable, cRight, pivot);
+    WFSplitBucketListRight(node.buckets, node.pivotTable, cRight, pivot);
+    WeightSplitBucketListRight(node.buckets, node.pivotTable, cRight, pivot);
   }
 
   function {:opaque} CutoffNode(node: Node, lbound: Option<Key>, rbound: Option<Key>)
@@ -190,12 +186,10 @@ module ImplModelSplit {
     reveal_SplitChildRight();
     Pivots.WFSlice(child.pivotTable, 0, num_children_left - 1);
     Pivots.WFSuffix(child.pivotTable, num_children_left);
-    KMTable.Islice(child.buckets, 0, num_children_left);
-    KMTable.Isuffix(child.buckets, num_children_left);
-    WFBucketListSplitLeft(KMTable.ISeq(child.buckets), child.pivotTable, num_children_left);
-    WFBucketListSplitRight(KMTable.ISeq(child.buckets), child.pivotTable, num_children_left);
-    WeightBucketListSlice(KMTable.ISeq(child.buckets), 0, num_children_left);
-    WeightBucketListSuffix(KMTable.ISeq(child.buckets), num_children_left);
+    WFBucketListSplitLeft(child.buckets, child.pivotTable, num_children_left);
+    WFBucketListSplitRight(child.buckets, child.pivotTable, num_children_left);
+    WeightBucketListSlice(child.buckets, 0, num_children_left);
+    WeightBucketListSuffix(child.buckets, num_children_left);
     assert WFNode(SplitChildRight(child, num_children_left));
     assert WFNode(SplitChildLeft(child, num_children_left));
   }
@@ -220,7 +214,7 @@ module ImplModelSplit {
   requires fused_parent.children.Some?
   {
     var pivots := Sequences.insert(fused_parent.pivotTable, pivot, slot_idx);
-    var buckets := KMTable.splitKMTInList(fused_parent.buckets, slot_idx as uint64, pivot);
+    var buckets := SplitBucketInList(fused_parent.buckets, slot_idx, pivot);
     Node(
       pivots,
       Some(replace1with2(fused_parent.children.value, left_childref, right_childref, slot_idx)),
@@ -228,7 +222,7 @@ module ImplModelSplit {
     )
   }
 
-  lemma SplitParentCorrect(rootBucket: Bucket, parentref: BT.G.Reference, fused_parent: Node, pivot: Key, slot_idx: int, left_childref: BT.G.Reference, right_childref: BT.G.Reference)
+  lemma SplitParentCorrect(parentref: BT.G.Reference, fused_parent: Node, pivot: Key, slot_idx: int, left_childref: BT.G.Reference, right_childref: BT.G.Reference)
   requires WFNode(fused_parent)
   requires BT.WFNode(INode(fused_parent))
   requires 0 <= slot_idx < |fused_parent.buckets|
@@ -238,25 +232,16 @@ module ImplModelSplit {
   ensures
     && var res := SplitParent(fused_parent, pivot, slot_idx, left_childref, right_childref);
     && WFNode(res)
-    && var inode := if parentref == BT.G.Root() then INodeRoot(fused_parent, rootBucket) else INode(fused_parent);
-    && var inode' := if parentref == BT.G.Root() then INodeRoot(res, rootBucket) else INode(res);
+    && var inode := INode(fused_parent);
+    && var inode' := INode(res);
     && inode' == BT.SplitParent(inode, pivot, slot_idx, left_childref, right_childref)
-    && WeightBucketList(KMTable.ISeq(res.buckets)) == WeightBucketList(KMTable.ISeq(fused_parent.buckets))
+    && WeightBucketList(res.buckets) == WeightBucketList(fused_parent.buckets)
   {
     var res := SplitParent(fused_parent, pivot, slot_idx, left_childref, right_childref);
-    WFSplitBucketInList(KMTable.ISeq(fused_parent.buckets), slot_idx, pivot, fused_parent.pivotTable);
-    WeightSplitBucketInList(KMTable.ISeq(fused_parent.buckets), slot_idx, pivot);
+    WFSplitBucketInList(fused_parent.buckets, slot_idx, pivot, fused_parent.pivotTable);
+    WeightSplitBucketInList(fused_parent.buckets, slot_idx, pivot);
     assert WFNode(res);
     assert INode(res) == BT.SplitParent(INode(fused_parent), pivot, slot_idx, left_childref, right_childref);
-
-    if (parentref == BT.G.Root()) {
-      BucketListFlushSplitInList(
-        rootBucket,
-        KMTable.ISeq(fused_parent.buckets),
-        fused_parent.pivotTable,
-        slot_idx,
-        pivot);
-    }
   }
 
   lemma lemmaSplitParentValidReferences(fused_parent: BT.G.Node, pivot: Key, slot_idx: int, left_childref: BT.G.Reference, right_childref: BT.G.Reference, graph: map<BT.G.Reference, seq<BT.G.Reference>>)
@@ -412,7 +397,7 @@ module ImplModelSplit {
             var s' := write(k, s2, parentref, split_parent);
 
             lemmaSplitChild(child, num_children_left);
-            SplitParentCorrect(s.rootBucket, parentref, fused_parent, pivot, slot, left_childref.value, right_childref.value);
+            SplitParentCorrect(parentref, fused_parent, pivot, slot, left_childref.value, right_childref.value);
 
             lemmaBlockPointsToValidReferences(k, s, childref);
             assert BC.BlockPointsToValidReferences(INode(fused_child), IIndirectionTable(s.ephemeralIndirectionTable).graph);
@@ -421,19 +406,16 @@ module ImplModelSplit {
             writeNewRefIsAlloc(k, s, left_childref.value, left_child);
             writeNewRefIsAlloc(k, s1, right_childref.value, right_child);
 
-            var inodeFusedParent := if parentref == BT.G.Root() then INodeRoot(fused_parent, s.rootBucket) else INode(fused_parent);
-            var inodeSplitParent := if parentref == BT.G.Root() then INodeRoot(split_parent, s.rootBucket) else INode(split_parent);
+            var inodeFusedParent := INode(fused_parent);
+            var inodeSplitParent := INode(split_parent);
 
             lemmaBlockPointsToValidReferences(k, s, parentref);
             assert BC.BlockPointsToValidReferences(inodeFusedParent, IIndirectionTable(s2.ephemeralIndirectionTable).graph);
             lemmaSplitParentValidReferences(inodeFusedParent, pivot, slot, left_childref.value, right_childref.value, IIndirectionTable(s2.ephemeralIndirectionTable).graph);
 
-            writeCorrectWithRootBucket(k, s2, parentref, split_parent);
-          
             reveal_SplitChildLeft();
             reveal_SplitChildRight();
 
-            assert WFBuckets(child.buckets);
             assert INode(child) == BT.CutoffNode(INode(fused_child), lbound, ubound);
             assert 1 <= num_children_left < |child.buckets|;
 
